More updates to open semantics preservation from earlier today

sepcomp/open_safety_preservation.v
@@ -20,6 +20,12 @@ Require Import sepcomp.extspec.
 
 Import SM_simulation.
 
+Definition corestep_fun {G C : Type} (sem : @CoopCoreSem G C) :=
+  forall (m m' m'' : mem) ge c c' c'',
+  corestep sem ge c m c' m' -> 
+  corestep sem ge c m c'' m'' -> 
+  c'=c'' /\ m'=m''.
+
 Definition target_accessible mu m tm args b ofs :=
   Mem.valid_block tm b /\ 
   (locBlocksTgt mu b=false -> 
@@ -101,20 +107,103 @@ Inductive trace_match_state :
   match_state cd j c m d tm -> 
   trace_match_state cd j (z,tr,c) m (z,ttr,d) tm. 
 
-Variables 
-(SRC_DET : corestep_fun source)
-(TGT_DET : corestep_fun target).
+Variables (SRC_DET : corestep_fun source) (TGT_DET : corestep_fun target).
 
 Notation tr_source := (TraceSemantics.coopsem z_init source spec).
 Notation tr_target := (TraceSemantics.coopsem z_init target spec).
 
-Lemma corestep_plus_match {c m d tm c' m' cd j} :
-  corestep_plus source geS c m c' m' -> 
+Arguments core_diagram : default implicits.
+
+Lemma corestepN_match {c m d tm c' m' cd j n} :
+  corestepN source geS n c m c' m' -> 
+  match_state cd j c m d tm -> 
+  exists d' tm' cd' j' n', 
+    corestepN target geT n' d tm d' tm'
+    /\ match_state cd' j' c' m' d' tm'.
+Proof.
+revert cd j c m d tm; induction n; simpl; intros cd j c m d tm.
+inversion 1; subst.
+intros MATCH; exists d, tm, cd, j, O; split; simpl; auto.
+intros [c2 [m2 [STEP STEPN]]] MATCH.
+generalize STEP as STEP'; intro.
+eapply core_diagram in STEP; eauto.
+destruct STEP as [d2 [tm2 [cd2 [j2 [? [? [? [MATCH2 [? [? TSTEPN]]]]]]]]]].
+assert (exists n', corestepN target geT n' d tm d2 tm2) as [n' TSTEPN'].
+{ destruct TSTEPN as [[n' X]|[[n' X] _]].
+  exists (S n'); auto.
+  exists n'; auto. }
+assert (STEPN': corestepN source geS (S O) c m c2 m2).
+{ simpl; exists c2, m2; split; auto. }
+destruct (IHn _ _ _ _ _ _ STEPN MATCH2)
+  as [d'' [tm'' [cd'' [j'' [n'' [TSTEPN'' MATCH']]]]]].
+exists d'', tm'', cd'', j'', (plus n' n''); split; auto.
+rewrite corestepN_add; exists d2, tm2; split; auto.
+Qed.
+
+Lemma yielded_src_target {cd j c d m tm} :
+  match_state cd j c m d tm -> 
+  TraceSemantics.yielded source c -> 
+  TraceSemantics.yielded target d.
+Proof.
+intros MATCH [[ef [sig [args X]]]|[rv X]].
+eapply core_at_external in MATCH; eauto.
+destruct MATCH as [? [? [? ?]]]; left.
+exists ef, sig, x; auto.
+eapply core_halted in MATCH; eauto.
+destruct MATCH as [? [? [? ?]]].
+right; exists x; auto.
+Qed.
+
+Definition my_P := fun (x: data) => 
+   forall (j : SM_Injection) c m d tm c' m' n,
+   corestepN source geS n c m c' m' -> 
+   TraceSemantics.yielded source c' -> 
+   match_state x j c m d tm -> 
+   exists d' tm' cd' j', 
+     corestep_plus target geT d tm d' tm'
+     /\ match_state cd' j' c' m' d' tm'.
+
+Lemma corestep_yield_match {c m d tm c' m' cd j n} :
+  corestepN source geS n c m c' m' -> 
+  TraceSemantics.yielded source c' -> 
   match_state cd j c m d tm -> 
   exists d' tm' cd' j', 
     corestep_plus target geT d tm d' tm'
     /\ match_state cd' j' c' m' d' tm'.
-Admitted.
+Proof.
+assert (my_well_founded_induction
+     : (forall x, (forall y, ord y x -> my_P y) -> my_P x) ->
+       forall a, my_P a)
+  by (apply well_founded_induction; destruct sim; auto).
+unfold my_P in my_well_founded_induction.
+revert cd j c m d tm c' m' n.
+apply my_well_founded_induction; auto.
+intros x IH j c m d tm c' m' n.
+
+
+
+intros X Y M; destruct X as [c2 [m2 [STEP STEPN]]].
+generalize STEP as STEP'; intro.
+eapply core_diagram in STEP; eauto.
+destruct STEP 
+  as [d2 [tm2 [? [? [? [? [? [M2 [? [? 
+     [[n2 P]|[[n2 S] ORD]]]]]]]]]]]]. 
+{ (* target plus case *)
+  eapply corestepN_match in STEPN; eauto.
+  destruct STEPN as [d' [tm' [cd' [j' [n' [TSTEPN MATCH']]]]]].
+  exists d', tm', cd', j'; split; auto.
+  destruct P as [d3 [tm3 [? ?]]].
+  exists (plus n2 n'); exists d3, tm3; split; auto.
+  rewrite corestepN_add; exists d2, tm2; split; auto. }
+{ (* target star case *)
+  destruct n2. inv S.
+  generalize (IH _ ORD _ _ _ _ _ _ _ PLUS M).
+
+
+  assert (PLUS: corestep_plus source geS c m c' m')
+    by (exists n, c2, m2; split; auto).
+
+  
 
 Lemma REACH_mono':
   forall B1 B2 : block -> bool,
@@ -274,20 +363,6 @@ unfold restrict; rewrite H5; auto.
 intros INJ'.
 unfold restrict.
 rewrite INJ'; destruct (DomSrc j b); auto.
-Qed.
-
-Lemma yielded_source_yielded_target {cd j c d m tm} :
-  match_state cd j c m d tm -> 
-  TraceSemantics.yielded source c -> 
-  TraceSemantics.yielded target d.
-Proof.
-intros MATCH [[ef [sig [args X]]]|[rv X]].
-eapply core_at_external in MATCH; eauto.
-destruct MATCH as [? [? [? ?]]]; left.
-exists ef, sig, x; auto.
-eapply core_halted in MATCH; eauto.
-destruct MATCH as [? [? [? ?]]].
-right; exists x; auto.
 Qed.
 
 Arguments match_sm_wd : default implicits.
